ZFC_utils.thy
@@ -1,0 +1,55 @@
+section "ZFC utilities"
+
+theory ZFC_utils
+  imports Main
+    "ZFC_in_HOL.ZFC_Typeclasses"
+begin
+
+
+
+definition to_V :: "'a::embeddable \<Rightarrow> V" where
+"to_V \<equiv> SOME f. inj f \<and> ((\<exists>(g::'a\<Rightarrow>V). inj g \<and> small (range g)) \<longrightarrow> small (range f))"
+
+definition from_V :: "V \<Rightarrow> 'a::embeddable" where
+"from_V \<equiv> the_inv to_V"
+
+
+lemma to_V_property: "inj (to_V::'a::embeddable\<Rightarrow>V) \<and> ((\<exists>g::'a\<Rightarrow>V. inj g \<and> small (range g)) \<longrightarrow> small (range (to_V::'a::embeddable\<Rightarrow>V)))"
+proof -
+
+  have "\<exists>f::'a\<Rightarrow>V. inj f"
+    using ex_inj by simp
+
+
+  hence ex: "\<exists>f::'a\<Rightarrow>V. inj f \<and> ((\<exists>g::'a\<Rightarrow>V. inj g \<and> small (range g)) \<longrightarrow> small (range f))"
+    by blast
+
+
+  from someI_ex[OF ex, simplified to_V_def[symmetric]] [[show_sorts]]
+  show "inj (to_V::'a\<Rightarrow>V) \<and> ((\<exists>g::'a\<Rightarrow>V. inj g \<and> small (range g)) \<longrightarrow> small (range (to_V::'a::embeddable\<Rightarrow>V)))"
+    by auto
+qed
+
+lemma to_V_inj: "inj to_V"
+  using to_V_property by auto
+
+
+lemma to_V_use_inj: "to_V x = to_V y \<Longrightarrow> x = y"
+  by (meson injD to_V_inj)
+
+
+lemma from_V_rev[simp]: 
+"from_V (to_V x) = x"
+  by (simp add: from_V_def the_inv_f_f to_V_inj)
+
+lemma to_V_small: "small (range (to_V::'a::small\<Rightarrow>V))"
+  using to_V_property down small by blast 
+
+lemma show_small_type_class:
+  assumes "\<exists>V_of::'a\<Rightarrow>V. inj V_of \<and> small (range V_of)"
+  shows "OFCLASS('a, small_class)"
+  by (standard, use assms small_iff in force)
+
+\<comment> \<open>TODO add methods to derive instances \<close>
+
+end
